src/3d/Options.fsti
@@ -35,3 +35,5 @@ val get_check_hashes : unit -> ML (option check_hashes_t)
 val get_save_hashes : unit -> ML bool
 
 val get_check_inplace_hashes : unit -> ML (list string)
+
+val get_equate_types_list : unit -> ML (list (string & string))
